

Goal: compute the coefficients  $\int_T (v_{\text{CR}} - J_2 v_{\text{CR}}) \Phi_{T,P}$  for every triangle T and vertex P.

Given:

$$b_F := 6 \prod_{P \in \mathcal{V}(F)} \lambda_P$$

$$\Phi_{T,P} := \sqrt{\frac{20}{27|T|}} \left( (\sqrt{7} + 1) - 3\sqrt{7}\lambda_P \right) =: \alpha - \beta\lambda_P$$

$$\begin{aligned} v_{\text{CR}} &= x_1\psi_1 + x_2\psi_2 + x_3\psi_3 \\ &= x_1(1 - 2\lambda_1) + x_2(1 - 2\lambda_2) + x_3(1 - 2\lambda_3) \\ &= \underbrace{(x_1 + x_2 + x_3)}_{=: \chi} - 2(x_1\lambda_1 + x_2\lambda_2 + x_3\lambda_3) \end{aligned}$$

$$\begin{aligned} J_2 v_{\text{CR}} &= J_1 v_{\text{CR}} + \sum_{F \in \mathcal{F}(\Omega)} \int_F (v_{\text{CR}} - J_1 v_{\text{CR}}) b_F \\ &= a_1\lambda_1 + a_2\lambda_2 + a_3\lambda_3 + 6(b_1\lambda_2\lambda_3 + b_2\lambda_1\lambda_3 + b_3\lambda_1\lambda_2) \end{aligned}$$

Calculate:

$$\begin{aligned} v_{\text{CR}} \Phi_{T,P} &= [\chi - 2(x_1\lambda_1 + x_2\lambda_2 + x_3\lambda_3)][\alpha - \beta\lambda_P] \\ &= \chi\alpha - \chi\beta\lambda_P - 2\alpha(x_1\lambda_1 + x_2\lambda_2 + x_3\lambda_3) + 2\beta(x_1\lambda_1\lambda_P + x_2\lambda_2\lambda_P + x_3\lambda_3\lambda_P) \\ J_2 v_{\text{CR}} \Phi_{T,P} &= [a_1\lambda_1 + a_2\lambda_2 + a_3\lambda_3 + 6(b_1\lambda_2\lambda_3 + b_2\lambda_1\lambda_3 + b_3\lambda_1\lambda_2)][\alpha - \beta\lambda_P] \\ &= \alpha(a_1\lambda_1 + a_2\lambda_2 + a_3\lambda_3 + 6(b_1\lambda_2\lambda_3 + b_2\lambda_1\lambda_3 + b_3\lambda_1\lambda_2)) \\ &\quad - \beta(a_1\lambda_1\lambda_P + a_2\lambda_2\lambda_P + a_3\lambda_3\lambda_P) \\ &\quad - 6\beta(b_1\lambda_2\lambda_3\lambda_P + b_2\lambda_1\lambda_3\lambda_P + b_3\lambda_1\lambda_2\lambda_P) \end{aligned}$$

using  $\int_T \lambda_1^\alpha \lambda_2^\beta \lambda_3^\gamma = 2|T| \frac{\alpha!\beta!\gamma!}{(2+\alpha+\beta+\gamma)!}$  we get the following cases:

P0:  $\int_T 1 = |T|$

P1:  $\int_T \lambda_j = \frac{1}{3}|T|$

P2:  $\int_T \lambda_i \lambda_j = |T| \begin{cases} \frac{1}{12} & \text{for } i \neq j \\ \frac{1}{6} & \text{for } i = j \\ \frac{1}{60} & \text{for } i \neq j \neq k \end{cases}$

P3:  $\int_T \lambda_i \lambda_j \lambda_k = |T| \begin{cases} \frac{1}{30} & \text{for } i \neq j = k \\ \frac{1}{10} & \text{for } i = j = k \end{cases}$

collect the coefficients of  $v_{\text{CR}} - J_2 v_{\text{CR}}$ :

P0:  $\chi\alpha$

P1:  $\chi(-\beta - 2\alpha) - \alpha(a_1 + a_2 + a_3)$

P2 case 1:  $2\beta(x_{P+1} + x_{P+2}) - 6\alpha(b_1 + b_2 + b_3) + \beta(a_{P+1} + a_{P+2})$

P2 case 2:  $\beta(2x_P + a_P)$

P3 case 1:  $6\beta b_P$

P3 case 2:  $6\beta(b_{P+1} + b_{P+2})$

P3 case 3: 0

combine for the final formula:

$$\begin{aligned}
\int_T (v_{\text{CR}} - J_2 v_{\text{CR}}) \Phi_{\text{T,P}} &= |T| \left[ \chi \alpha \right. \\
&\quad - \frac{1}{3} (\chi (\beta + 2\alpha) + \alpha a_{\text{sum}}) \\
&\quad + \frac{1}{12} (2\beta x_{\text{other}} - 6\alpha b_{\text{sum}} + \beta a_{\text{other}}) \\
&\quad + \frac{1}{6} \beta (2x_P + a_P) \\
&\quad + \frac{1}{60} 6\beta b_P \\
&\quad \left. + \frac{1}{30} 6\beta b_{\text{other}} \right] \\
&= |T| \left[ \frac{1}{3} (\chi (\alpha - \beta) - \alpha a_{\text{sum}}) + \frac{1}{12} (\beta (2x_{\text{other}} + a_{\text{other}}) - 6\alpha b_{\text{sum}}) \right. \\
&\quad \left. + \frac{1}{6} \beta (2x_P + a_P) + \frac{1}{10} \beta b_P + \frac{1}{5} \beta b_{\text{other}} \right]
\end{aligned}$$